compiler/backend/semantics/labSemScript.sml
@@ -1,10 +1,13 @@
 open preamble labLangTheory;
-local open wordSemTheory alignmentTheory targetSemTheory in end;
+local open alignmentTheory targetSemTheory in end;
 
 val _ = new_theory"labSem";
 
 (* TODO: awaiting HOL issue #168 *)
 val () = Parse.temp_type_abbrev ("prog", ``:('a labLang$sec) list``);
+
+val _ = Datatype `
+  word_loc = Word ('a word) | Loc num num `;
 
 val _ = Datatype `
   word8_loc = Byte word8 | LocByte num num num`;
